snap

io/DM.MIO.fst
@@ -1,15 +1,23 @@
 module DM.MIO
 
-open Free.IO
-open Free.IO.Call
+open FStar.Tactics
+
+open IO.Sig
+open IO.Sig.Call
 open DM.IO
 
-effect MIO
-  (a:Type) =
-  IOwp a (fun _ p -> forall res le. p res le)
+let trivial_wp a : hist a =
+  fun p _ -> forall l r. p l r
+
+effect MIO (a:Type) = IOwp a (trivial_wp a)
+#set-options "--print_implicits"
+let lemma_trivial_wp_theta (cmd:io_cmds) (argz:io_sig.args cmd) :
+  Lemma (trivial_wp (io_sig.res cmd argz) `hist_ord #_ #(io_sig.res cmd argz)` dm_io_theta (io_call cmd argz)) = admit ()
 
 let unsafe_cmd
   (cmd : io_cmds)
-  (argz : io_args cmd) :
-  MIO (io_resm cmd) =
-    IOwp?.reflect(fun _ _ -> io_call cmd argz)
+  (argz : io_sig.args cmd) :
+  MIO (io_sig.res cmd argz) =
+    IOwp?.reflect (
+      lemma_trivial_wp_theta cmd argz;
+      io_call cmd argz)
